theories/CodegenWasm/LambdaANF_to_Wasm_correct.v
@@ -3030,30 +3030,15 @@ Proof.
    }
 Qed.
 
-Lemma numOf_fundefs_length :
-  forall f0 fns,
-  (fix iter (fds : fundefs) : error (seq.seq wasm_function) :=
-     match fds with
-     | Fcons x _ xs e fds' =>
-         match translate_function nenv cenv fenv x xs e with
-         | Err t => fun _ : wasm_function -> error (seq.seq wasm_function) => Err t
-         | Ret a => fun m2 : wasm_function -> error (seq.seq wasm_function) => m2 a
-         end
-           (fun fn : wasm_function =>
-            match iter fds' with
-            | Err t =>
-                fun _ : seq.seq wasm_function -> error (seq.seq wasm_function) => Err t
-            | Ret a =>
-                fun m2 : seq.seq wasm_function -> error (seq.seq wasm_function) => m2 a
-            end (fun following : seq.seq wasm_function => Ret (fn :: following)%SEQ))
-     | Fnil => Ret []
-     end) f0 = Ret fns -> numOf_fundefs f0 = length fns.
+Lemma translate_functions_numOf_fundefs_length : forall fds fns,
+  translate_functions nenv cenv fenv fds = Ret fns ->
+  numOf_fundefs fds = length fns.
 Proof.
-  induction f0; intros. 2: { now inv H. }
+  induction fds; intros. 2: { now inv H. }
+  simpl in H.
   destruct (translate_function nenv cenv fenv v l e). inv H.
-  destruct (_ f0). inv H. destruct fns; inv H. cbn. now rewrite -IHf0.
+  destruct (translate_functions _ _ _ fds). inv H. destruct fns; inv H. cbn. now rewrite -IHfds.
 Qed.
-
 
 Lemma collect_function_vars_length_numOf_fundefs_eq : forall fds e,
   length (collect_function_vars (Efun fds e)) = numOf_fundefs fds.
@@ -3306,7 +3291,6 @@ Proof.
     cbn. apply IHbrs in H5. now rewrite H5.
 Qed.
 
-
 Lemma create_case_nested_if_chain_repr_case_boxed : forall v brs es,
     repr_case_boxed v brs es ->
     create_case_nested_if_chain true v brs = es.
@@ -3319,7 +3303,6 @@ Proof.
     cbn. apply IHbrs in H5. now rewrite H5.
 Qed.
 
-
 Lemma lholed_nested_label : forall k (lh : lholed k) es,
   exists k' (lh' : lholed k'),
   lfill lh [:: AI_label 0 [::] es] = lfill lh' es.
@@ -3331,7 +3314,6 @@ Proof.
     eexists. exists (LH_rec l n l0 lh' l1). cbn.
     now rewrite Heq.
 Qed.
-
 
 Lemma and_of_odd_and_1_1 : forall n,
     (-1 < Z.of_nat (Pos.to_nat (2 * n + 1)) < Wasm_int.Int32.modulus)%Z ->
@@ -3510,7 +3492,6 @@ Proof.
     }
   }
 Qed.
-
 
 Lemma boxed_nested_if_chain_reduces:
   forall cl fAny y t vs e addr v lenv brs1 brs2 e1' (hs : host_state) (sr : store_record) (f : frame),
@@ -6109,191 +6090,88 @@ Proof.
   reflexivity.
 Qed.
 
-
-Lemma translate_functions_exists_original_fun : forall fds fds'' fns wasmFun e,
+Lemma translate_functions_exists_original_fun : forall fds fds'' fns wasmFun e eAny,
   NoDup (collect_function_vars (Efun fds e)) ->
-  (fix iter (fds : fundefs) : error (seq.seq wasm_function) :=
-               match fds with
-               | Fcons x _ xs e fds' =>
-                   match
-                     translate_function nenv cenv (create_fname_mapping (Efun fds'' e)) x
-                       xs e
-                   with
-                   | Err t => fun _  : wasm_function -> error (seq.seq wasm_function) => Err t
-                   | Ret a => fun m2 : wasm_function -> error (seq.seq wasm_function) => m2 a
-                   end
-                     (fun fn : wasm_function =>
-                      match iter fds' with
-                      | Err t =>
-                          fun _ : seq.seq wasm_function -> error (seq.seq wasm_function) =>
-                          Err t
-                      | Ret a =>
-                          fun m2 : seq.seq wasm_function -> error (seq.seq wasm_function) =>
-                          m2 a
-                      end (fun following : seq.seq wasm_function => Ret (fn :: following)%SEQ))
-               | Fnil => Ret []
-               end) fds = Ret fns ->
-   In wasmFun fns ->
-   exists f t ys e, find_def f fds = Some (t, ys, e) /\ match wasmFun.(type) with
-                                                        | Tf args _ => length ys = length args
-                                                        end.
+  translate_functions nenv cenv (create_fname_mapping (Efun fds'' eAny)) fds = Ret fns ->
+  In wasmFun fns ->
+  exists f t ys e, find_def f fds = Some (t, ys, e) /\ match wasmFun.(type) with
+                                                       | Tf args _ => length ys = length args
+                                                       end.
 Proof.
-  induction fds; intros fds'' fns wasmFun e' Hnodup Htrans Hin. 2: { inv Htrans. inv Hin. }
-  destruct (translate_function nenv cenv
-        (create_fname_mapping (Efun _ e)) v l
-        e) eqn:transF. inv Htrans. cbn.
-  destruct ((fix iter (fds : fundefs) : error (seq.seq wasm_function) :=
-              match fds with
-              | Fcons x _ xs e0 fds' =>
-                  match
-                    translate_function nenv cenv
-                      (create_fname_mapping (Efun _ e0)) x xs e0
-                  with
-                  | Err t =>
-                      fun _ : wasm_function -> error (seq.seq wasm_function) => Err t
-                  | Ret a =>
-                      fun m2 : wasm_function -> error (seq.seq wasm_function) => m2 a
-                  end
-                    (fun fn : wasm_function =>
-                     match iter fds' with
-                     | Err t =>
-                         fun _ : seq.seq wasm_function ->
-                               error (seq.seq wasm_function) => Err t
-                     | Ret a => fun m2 : seq.seq wasm_function ->
-                                error (seq.seq wasm_function) => m2 a
-                     end
-                       (fun following : seq.seq wasm_function =>
-                        Ret (fn :: following)%SEQ))
-              | Fnil => Ret []
-              end) fds) eqn:Htra; inv Htrans. destruct Hin.
-  { (* wasmFun is first fn *) subst w.
+  induction fds; intros fds'' fns wasmFun e' eAny Hnodup Htrans Hin. 2: { inv Htrans. inv Hin. }
+  simpl in Htrans.
+  destruct (translate_function nenv cenv (create_fname_mapping (Efun _ _)) v l e) eqn:transF. inv Htrans.
+  cbn. destruct (translate_functions _ _ _ ) eqn:Htra; inv Htrans. destruct Hin.
+  - (* wasmFun is first fn *) subst w.
     exists v, f, l, e. destruct (M.elt_eq); last contradiction.
     split; auto.
     unfold translate_function in transF.
-    destruct (translate_exp _ _ _ _) eqn:HtransE. inv transF.
     destruct (translate_var _ _ _ _) eqn:HtransFvar. inv transF.
-    inv transF. cbn. now rewrite map_length. }
-  { (* wasmFun is not first fn *)
-    eapply IHfds in H; auto. 2: { now inv Hnodup. }
-    { destruct H as [f' [t' [ys' [e'' [Hfdef Hty]]]]].
-      exists f', t', ys', e''. split; auto. rewrite -Hfdef.
-      destruct (M.elt_eq f' v); auto. subst v. exfalso.
-      inv Hnodup. apply H1. clear H2. cbn.
-      eapply find_def_in_collect_function_vars. eapply notNone_Some; eauto.
-    }
-    eassumption.
-  }
-  Unshelve. all: assumption.
+    destruct (translate_exp _ _ _ _) eqn:HtransE. inv transF.
+    inv transF. cbn. now rewrite map_length.
+  - (* wasmFun is not first fn *)
+    eapply IHfds in H; eauto. 2: { now inv Hnodup. }
+    destruct H as [f' [t' [ys' [e'' [Hfdef Hty]]]]].
+    exists f', t', ys', e''. split; auto. rewrite -Hfdef.
+    destruct (M.elt_eq f' v); auto. subst v. exfalso.
+    inv Hnodup. apply H1. clear H2. cbn.
+    now eapply find_def_in_collect_function_vars.
+Unshelve. all: assumption.
 Qed.
 
-Lemma translate_funcs_fenv : forall fds fns fenv e,
+Lemma translate_functions_fenv : forall fds fns fenv e,
   map_injective fenv ->
-  (fix iter (fds : fundefs) :
-                 error (seq wasm_function) :=
-               match fds with
-               | Fcons x _ xs e0 fds' =>
-                   match
-                     translate_function nenv cenv fenv x xs e0
-                   with
-                   | Err t => fun _ : wasm_function -> error (seq wasm_function) => Err t
-                   | Ret a => fun m2 : wasm_function -> error (seq wasm_function) => m2 a
-                   end
-                     (fun fn : wasm_function =>
-                      match iter fds' with
-                      | Err t => fun _ : seq wasm_function -> error (seq wasm_function) => Err t
-                      | Ret a => fun m2 : seq wasm_function -> error (seq wasm_function) => m2 a
-                      end
-                        (fun following : seq wasm_function =>
-                         Ret (fn :: following)))
-               | Fnil => Ret [::]
-               end) fds = Ret fns ->
-
+  translate_functions nenv cenv fenv fds = Ret fns ->
   (forall x i, i < numOf_fundefs fds ->
                length fns = numOf_fundefs fds ->
                 (nth_error (collect_function_vars (Efun fds e)) i = Some x ->
                  option_map (fun f => fidx f) (nth_error fns i) = (fenv ! x))).
 Proof.
   induction fds; intros. 2:{ cbn in H1. lia. }
-  destruct fns. inv H2.
+  destruct fns. inv H2. simpl in H0.
   destruct (translate_function _ _ _ _ _ _) eqn:HtransF. inv H0.
-  destruct ((fix iter (fds : fundefs) : error (seq wasm_function) := _) fds) eqn:Hfix; inv H0.
+  destruct (translate_functions _ _ _ _) eqn:Hfns; inv H0.
   destruct i.
-  { (* i=0 *) cbn. inv H3.
-      unfold translate_function in HtransF.
-      destruct (translate_exp _ _ _ _ _). inv HtransF.
-      destruct (translate_var _ _ _ _) eqn:HtransV. inv HtransF. inv HtransF.
-      unfold translate_var in HtransV.
-      destruct (fenv ! x) eqn:HtransV'; inv HtransV. reflexivity.
-  }
-  { (* i=Si' *) cbn in H1. cbn.
-    eapply IHfds; eauto. lia. }
-  Unshelve. assumption.
+  - (* i=0 *)
+    cbn. inv H3.
+    unfold translate_function in HtransF.
+    destruct (translate_var _ _ _ _) eqn:HtransV. inv HtransF.
+    destruct (translate_exp _ _ _ _ _). inv HtransF. inv HtransF.
+    unfold translate_var in HtransV.
+    by destruct (fenv ! x) eqn:HtransV'; inv HtransV.
+  - (* i=Si' *)
+    cbn in H1. cbn.
+    eapply IHfds; eauto. lia.
+Unshelve. assumption.
 Qed.
 
-Lemma translate_funcs_idx_bounds : forall fds fns fenv min max,
+Lemma translate_functions_idx_bounds : forall fds fns fenv min max,
   (forall f f', fenv ! f = Some f' -> min <= f' < max) ->
   length fns = numOf_fundefs fds ->
-  (fix iter (fds : fundefs) :
-                 error (seq wasm_function) :=
-               match fds with
-               | Fcons x _ xs e0 fds' =>
-                   match
-                     translate_function nenv cenv fenv x xs e0
-                   with
-                   | Err t => fun _ : wasm_function -> error (seq wasm_function) => Err t
-                   | Ret a => fun m2 : wasm_function -> error (seq wasm_function) => m2 a
-                   end
-                     (fun fn : wasm_function =>
-                      match iter fds' with
-                      | Err t => fun _ : seq wasm_function -> error (seq wasm_function) => Err t
-                      | Ret a => fun m2 : seq wasm_function -> error (seq wasm_function) => m2 a
-                      end
-                        (fun following : seq wasm_function =>
-                         Ret (fn :: following)))
-               | Fnil => Ret [::]
-               end) fds = Ret fns ->
-
+  translate_functions nenv cenv fenv fds = Ret fns ->
   forall idx, In idx (map fidx fns) -> min <= idx < max.
 Proof.
-  induction fds; intros. 2:{ inv H1. contradiction. }
-  destruct fns. inv H0.
-  destruct (translate_function _ _ _ _ _ _) eqn:HtransF. inv H1.
-  destruct ((fix iter (fds : fundefs) : error (seq wasm_function) := _) fds) eqn:Hfix; inv H1.
-  destruct H2.
-  { (* i=0 *) subst.
-      unfold translate_function in HtransF.
-      destruct (translate_exp _ _ _ _ _). inv HtransF.
-      destruct (translate_var _ _ _ _) eqn:HtransV. inv HtransF. inv HtransF.
-      unfold translate_var in HtransV. cbn.
-      destruct (fenv ! v) eqn:HtransV'; inv HtransV. now apply H in HtransV'.
-  }
-  { (* i=Si' *) cbn in H1. cbn.
-    eapply IHfds; eauto. }
+  induction fds; intros ???? Hbounds Hlen Hfns ? Hin; last by inv Hfns.
+  destruct fns. inv Hin. simpl in Hfns.
+  destruct (translate_function _ _ _ _ _ _) eqn:HtransF. inv Hfns.
+  destruct (translate_functions _ _ _ fds) eqn:Hfix; inv Hfns.
+  destruct Hin.
+  - (* i=0 *)
+    subst. unfold translate_function in HtransF.
+    destruct (translate_var _ _ _ _) eqn:HtransV. inv HtransF.
+    destruct (translate_exp _ _ _ _ _). inv HtransF. inv HtransF.
+    unfold translate_var in HtransV. cbn.
+    destruct (fenv ! v) eqn:HtransV'; inv HtransV. now apply Hbounds in HtransV'.
+  - (* i=Si' *) cbn in Hlen. cbn.
+    by eapply IHfds; eauto.
 Qed.
 
-Lemma translate_funcs_increasing_fids : forall fds fns fenv e e',
+Lemma translate_functions_increasing_fids : forall fds fns fenv e e',
   fenv = create_fname_mapping e ->
   match e with Efun fds' _ => fds' = fds | _ => True end ->
   map_injective fenv ->
   NoDup (collect_function_vars (Efun fds e')) ->
-  (fix iter (fds : fundefs) :
-                 error (seq wasm_function) :=
-               match fds with
-               | Fcons x _ xs e0 fds' =>
-                   match
-                     translate_function nenv cenv
-                       (create_fname_mapping e) x xs e0
-                   with
-                   | Err t => fun _ : wasm_function -> error (seq wasm_function) => Err t
-                   | Ret a => fun m2 : wasm_function -> error (seq wasm_function) => m2 a
-                   end
-                     (fun fn : wasm_function =>
-                      match iter fds' with
-                      | Err t => fun _ : seq wasm_function -> error (seq wasm_function) => Err t
-                      | Ret a => fun m2 : seq wasm_function -> error (seq wasm_function) => m2 a
-                      end (fun following : seq wasm_function => Ret (fn :: following)))
-               | Fnil => Ret [::]
-               end) fds = Ret fns ->
+  translate_functions nenv cenv fenv fds = Ret fns ->
   (forall i j i' j', i > j -> nth_error (map (fun f => fidx f) fns) i = Some i' ->
                               nth_error (map (fun f => fidx f) fns) j = Some j' -> i' > j').
 Proof.
@@ -6302,18 +6180,18 @@ Proof.
   destruct (nth_error fns i) eqn:Hio. 2: inv Hi. cbn in Hi. inv Hi.
   destruct (nth_error fns j) eqn:Hjo. 2: inv Hj. cbn in Hj. inv Hj.
 
-  have Hlen := numOf_fundefs_length _ _ _ _ _ HtransFns. symmetry in Hlen.
+  have Hlen := translate_functions_numOf_fundefs_length _ _ _ _ _ HtransFns. symmetry in Hlen.
 
   assert (Hilen: i < numOf_fundefs fds). { rewrite -Hlen. now apply nth_error_Some. }
   have Hilen' := Hilen. rewrite <- (collect_function_vars_length_numOf_fundefs_eq _ e) in Hilen'.
   apply nth_error_Some in Hilen'. apply notNone_Some in Hilen'. destruct Hilen' as [v Hiv].
-  have Hi' := translate_funcs_fenv _ _ _ _ Hinj HtransFns _ _ Hilen Hlen Hiv.
+  have Hi' := translate_functions_fenv _ _ _ _ Hinj HtransFns _ _ Hilen Hlen Hiv.
   rewrite Hio in Hi'. cbn in Hi'.
 
   assert (Hjlen: j < numOf_fundefs fds). { rewrite -Hlen. now apply nth_error_Some. }
   have Hjlen' := Hjlen. rewrite <- (collect_function_vars_length_numOf_fundefs_eq _ e) in Hjlen'.
   apply nth_error_Some in Hjlen'. apply notNone_Some in Hjlen'. destruct Hjlen' as [v' Hjv'].
-  have Hj' := translate_funcs_fenv _ _ _ _ Hinj HtransFns _ _ Hjlen Hlen Hjv'.
+  have Hj' := translate_functions_fenv _ _ _ _ Hinj HtransFns _ _ Hjlen Hlen Hjv'.
   rewrite Hjo in Hj'. cbn in Hj'.
   symmetry in Hj', Hi'.
   destruct e; (try now inv Hjv'). subst f. clear HtransFns.
@@ -6329,12 +6207,10 @@ Proof.
   inv Hi''. inv Hj''. lia.
 Qed.
 
-
 Lemma increasing_list_fact_trans : forall n l i i' i'n,
   (forall i j i' j', i > j -> nth_error l i = Some i' ->
                               nth_error l j = Some j' -> i' > j') ->
   nth_error l i = Some i' ->
-
   nth_error l (i + n) = Some i'n -> i'n >= i' + n.
 Proof.
   induction n; intros. replace (i+0) with i in H1 by lia.
@@ -6372,7 +6248,7 @@ Proof.
     destruct H3 as [v Hv].
     have H' := increasing_list_fact_trans _ _ _ _ _ H Hv H1.
     apply H0 in Hv. lia. }
-    lia.
+  lia.
 Qed.
 
 Lemma fns_fidx_nth_error_fidx : forall fns func j,
@@ -6405,34 +6281,16 @@ Proof.
   assert (i=j) by lia. now subst i.
 Qed.
 
-
-Lemma translate_funcs_NoDup : forall fds fns fenv e e',
+Lemma translate_functions_NoDup : forall fds fns fenv e e',
   fenv = create_fname_mapping e ->
   match e with Efun fds' _ => fds' = fds | _ => True end ->
   map_injective fenv ->
   NoDup (collect_function_vars (Efun fds e')) ->
-  (fix iter (fds : fundefs) :
-                 error (seq wasm_function) :=
-               match fds with
-               | Fcons x _ xs e0 fds' =>
-                   match
-                     translate_function nenv cenv
-                       (create_fname_mapping e) x xs e0
-                   with
-                   | Err t => fun _ : wasm_function -> error (seq wasm_function) => Err t
-                   | Ret a => fun m2 : wasm_function -> error (seq wasm_function) => m2 a
-                   end
-                     (fun fn : wasm_function =>
-                      match iter fds' with
-                      | Err t => fun _ : seq wasm_function -> error (seq wasm_function) => Err t
-                      | Ret a => fun m2 : seq wasm_function -> error (seq wasm_function) => m2 a
-                      end (fun following : seq wasm_function => Ret (fn :: following)))
-               | Fnil => Ret [::]
-               end) fds = Ret fns ->
+  translate_functions nenv cenv fenv fds = Ret fns ->
   NoDup (map (fun f => fidx f) fns).
 Proof.
   intros ? ? ? ? ? ? Hfds Hinj Hnodup HtransFns. subst fenv.
-  have H' := translate_funcs_increasing_fids _ _ _ _ _ Logic.eq_refl Hfds Hinj Hnodup HtransFns.
+  have H' := translate_functions_increasing_fids _ _ _ _ _ Logic.eq_refl Hfds Hinj Hnodup HtransFns.
   apply NoDup_nth_error. intros ? ? HiLen Heq.
   destruct (Nat.eq_dec i j); auto. exfalso.
   apply nth_error_Some in HiLen. apply notNone_Some in HiLen. destruct HiLen as [v Hv].
@@ -6445,26 +6303,9 @@ Proof.
   have Hcontra := H' _ _ _ _ Hgt Hv Heq. lia.
 Qed.
 
-Lemma translate_funcs_find_def : forall fds f fns t ys e fenv,
+Lemma translate_functions_find_def : forall fds f fns t ys e fenv,
   NoDup (collect_function_vars (Efun fds e)) ->
-  (fix iter (fds : fundefs) :  error (seq wasm_function) :=
-               match fds with
-               | Fcons x _ xs e0 fds' =>
-                   match
-                     translate_function nenv cenv fenv x xs e0
-                   with
-                   | Err t => fun _ : wasm_function -> error (seq wasm_function) => Err t
-                   | Ret a => fun m2 : wasm_function -> error (seq wasm_function) => m2 a
-                   end
-                     (fun fn : wasm_function =>
-                      match iter fds' with
-                      | Err t => fun _ : seq wasm_function -> error (seq wasm_function) => Err t
-                      | Ret a => fun m2 : seq wasm_function -> error (seq wasm_function) => m2 a
-                      end
-                        (fun following : seq wasm_function =>
-                         Ret (fn :: following)))
-               | Fnil => Ret [::]
-               end) fds = Ret fns ->
+  translate_functions nenv cenv fenv fds = Ret fns ->
   find_def f fds = Some (t, ys, e) ->
   (forall f t ys e, find_def f fds = Some (t, ys, e) -> correct_cenv_of_exp cenv e) ->
   exists idx e' locs ftype func, repr_funvar fenv nenv f idx /\
@@ -6475,25 +6316,25 @@ Lemma translate_funcs_find_def : forall fds f fns t ys e fenv,
     repr_expr_LambdaANF_Wasm cenv fenv nenv e e'
      (lenv := create_local_variable_mapping (ys ++ collect_local_variables e)).
 Proof.
-  induction fds; intros ? ? ? ? ? ? Hnodup HtransFns HfDef HcorrCenv. 2: inv HfDef.
+  induction fds; intros ? ? ? ? ? ? Hnodup HtransFns HfDef HcorrCenv; last by inv HfDef.
+  simpl in HtransFns.
   destruct (translate_function _ _ _ _ _ _) eqn:Hf. inv HtransFns.
-  destruct (_ fds) eqn:Hfns; inv HtransFns.
+  destruct (translate_functions _ _ _ fds) eqn:Hfns; inv HtransFns.
   cbn in HfDef. destruct (M.elt_eq f0 v).
-  { (* f0=v *)
+  - (* f0=v *)
     inv HfDef.
     unfold translate_function in Hf.
-    destruct (translate_exp _ _ _ _ _) eqn:Hexp. inv Hf.
-    destruct (translate_var _ _ _ _) eqn:Hvar; inv Hf.
+    destruct (translate_var _ _ _ _) eqn:Hvar. inv Hf.
+    destruct (translate_exp _ _ _ _ _) eqn:Hexp; inv Hf.
     exists i, l. eexists. eexists. eexists.
-    split. { econstructor. eassumption. }
+    split. { now econstructor. }
     do 2! (split; try reflexivity).
     split. now left.
     cbn. rewrite map_repeat_eq.
     repeat (split; first reflexivity).
     eapply translate_exp_correct in Hexp; eauto. eapply HcorrCenv with (f:=v). cbn.
-    destruct (M.elt_eq v v); try contradiction. reflexivity.
-  }
-  { (* f0<>v *)
+    by destruct (M.elt_eq v v).
+  - (* f0<>v *)
     assert (Hnodup': NoDup (collect_function_vars (Efun fds e0))). {
       now inv Hnodup. }
     assert (HcorrCenv': (forall (f : var) (t : fun_tag) (ys : seq var) (e : exp),
@@ -6508,9 +6349,8 @@ Proof.
     destruct IH as [idx [e' [locs [type [func [? [? [? [? [? [? [? [? ?]]]]]]]]]]]]].
     inversion H.
     repeat eexists.
-    repeat (split; eauto).
-    rewrite -H3 in H8. eassumption.
-    now right. all: congruence. }
+    repeat (split; eauto). subst idx. eassumption.
+    now right. all: congruence.
 Qed.
 
 Theorem module_instantiate_INV_and_more_hold :
@@ -6529,17 +6369,20 @@ forall e eAny topExp fds num_funs module fenv main_lenv sr f exports,
   (* instantiate with the two imported functions *)
   instantiate host_function host_instance initial_store module
     [MED_func (Mk_funcidx 0); MED_func (Mk_funcidx 1)] (sr, (f_inst f), exports, None) ->
+
+  (* invariations hold initially *)
   INV fenv nenv _ sr f /\
   inst_funcs (f_inst f) = [:: 0, 1, 2, 3 & map (fun '(Mk_funcidx i) => i) (funcidcs num_funs 4)] /\
+  (* value relation holds for all funcs in fds *)
   (forall a errMsg, find_def a fds <> None ->
 	exists fidx : immediate,
 	  translate_var nenv fenv a errMsg = Ret fidx /\
 	  repr_val_LambdaANF_Wasm cenv fenv nenv host_function
 	    (Vfun (M.empty _) fds a) sr f (Val_funidx fidx)) /\
   (* pp_fn not called, discard *)
-   exists pp_fn e' fns, s_funcs sr = [:: FC_func_host (Tf [T_i32] []) hfn,
-                                         FC_func_host (Tf [T_i32] []) hfn,
-                                         pp_fn,
+  exists pp_fn e' fns, s_funcs sr = [:: FC_func_host (Tf [T_i32] []) hfn,
+                                        FC_func_host (Tf [T_i32] []) hfn,
+                                        pp_fn,
                        FC_func_native (f_inst f) (Tf [] [])
                          (map (fun _ : var => T_i32)
                             (collect_local_variables
@@ -6556,8 +6399,8 @@ forall e eAny topExp fds num_funs module fenv main_lenv sr f exports,
                                   | Tf args _ => Datatypes.length args
                                   end) []) (locals f0)
                             (body f0)) fns] /\
-   (* translation of e *)
-    translate_exp nenv cenv
+  (* translation of e *)
+  translate_exp nenv cenv
           (create_local_variable_mapping
              (collect_local_variables
                 match e with
@@ -6568,22 +6411,8 @@ forall e eAny topExp fds num_funs module fenv main_lenv sr f exports,
                            | _ => e
                            end = Ret e' /\
   (* translation of functions *)
-  match e with
-  | Efun fds _ =>
-    (fix iter (fds0 : fundefs) : error (seq.seq wasm_function) :=
-     match fds0 with
-     | Fcons x _ xs e fds' =>
-        match translate_function nenv cenv fenv x xs e with
-        | Err t => fun _ : wasm_function -> error (seq.seq wasm_function) => Err t
-        | Ret a => fun m2 : wasm_function -> error (seq.seq wasm_function) => m2 a
-        end
-      (fun fn : wasm_function =>
-        match iter fds' with
-        | Err t => fun _ : seq.seq wasm_function -> error (seq.seq wasm_function) => Err t
-        | Ret a => fun m2 : seq.seq wasm_function -> error (seq.seq wasm_function) => m2 a
-        end (fun following : seq.seq wasm_function => Ret (fn :: following)%SEQ))
-     | Fnil => Ret []
-     end) fds
+  match topExp with
+  | Efun fds _ => translate_functions nenv cenv fenv fds
   | _ => Ret []
   end = Ret fns.
 Proof.
@@ -6658,7 +6487,7 @@ Proof.
   assert (Hlen': length e_offs = length fns + 4). { now rewrite HeoffsLen -Hlen. }
   rewrite -Hlen' in HeoffsVals.
   assert (HlenMax: (Z.of_nat (Datatypes.length e_offs) < Wasm_int.Int32.modulus)%Z). {
-  apply numOf_fundefs_length in HtransFns.
+  apply translate_functions_numOf_fundefs_length in HtransFns.
   unfold max_num_functions in HfdsLength. simpl_modulus; cbn. lia. }
   assert (Hlen'': Datatypes.length e_offs = Datatypes.length (table_data t)) by lia.
   have H' := init_tabs_effect s' _ _ e_offs _ Heqts Hnone F2 F3 Logic.eq_refl HeoffsVals HlenMax Hlen''.
@@ -6677,7 +6506,7 @@ Proof.
   rewrite -map_map_seq in HallocModule. cbn in HallocModule.
   rewrite nth_list_function_types_map in HallocModule. 2: {
     intros wFun Hin. destruct e; inv HtopExp'; try by (inv HtransFns; inv Hin).
-    have H' := translate_functions_exists_original_fun _ _ _ _ _ Hnodup HtransFns Hin.
+    have H' := translate_functions_exists_original_fun _ _ _ _ _ _ Hnodup HtransFns Hin.
     destruct H' as [f'' [t'' [ys'' [e'' [Hdef Hty]]]]].
     destruct (type wFun).
     inv HeRestr. apply H2 in Hdef. lia. }
@@ -6719,7 +6548,7 @@ Proof.
      rewrite Hfuncs. cbn.
      rewrite map_length.
      destruct e; inv HtopExp'; try (inv HtransFns; simpl_modulus; cbn; lia).
-     erewrite <- numOf_fundefs_length; eauto.
+     erewrite <- translate_functions_numOf_fundefs_length; eauto.
      unfold max_num_functions in HfdsLength. simpl_modulus. cbn. lia. }
    split. (* inst_globs (f_inst f) no dups *)
    unfold INV_inst_globs_nodup. rewrite F0.
@@ -6739,7 +6568,7 @@ Proof.
       have H' := H.
       apply translate_fvar_fname_mapping in H'.
       destruct e; inv H. symmetry in HtopExp'; inv HtopExp'.
-      apply numOf_fundefs_length in HtransFns. rewrite HtransFns in H'.
+      apply translate_functions_numOf_fundefs_length in HtransFns. rewrite HtransFns in H'.
       apply nth_error_In with (n:=i). rewrite nth_error_map.
       rewrite HeoffsVals; try lia. cbn. f_equal.
       rewrite Wasm_int.Int32.Z_mod_modulus_id; try lia.
@@ -6761,14 +6590,14 @@ Proof.
   (* inst_funcs (f_inst f) *)
   { rewrite F3. repeat f_equal. intros. rewrite H2. reflexivity.
     destruct e; inv HtopExp'; inv HtransFns; auto.
-    symmetry. rewrite Hlen. cbn. eapply numOf_fundefs_length. eassumption. }
+    symmetry. rewrite Hlen. cbn. eapply translate_functions_numOf_fundefs_length. eassumption. }
   split. (* val relation holds for functions *)
   { intros. apply notNone_Some in H. destruct H as [[[v' ys'] e''] Hfd].
     assert (Hnodup' : NoDup (collect_function_vars (Efun fds e))). {
       replace (collect_function_vars (Efun fds e'')) with
               (collect_function_vars (Efun fds e0)) by reflexivity. assumption. }
 
-    have H' := translate_funcs_find_def _ _ _ _ _ e'' _ Hnodup' HtransFns Hfd HcenvCorrect.
+    have H' := translate_functions_find_def _ _ _ _ _ e'' _ Hnodup' HtransFns Hfd HcenvCorrect.
     destruct H' as [fidx [e''' [? [? [func [? [? [? [? [? [? [? [? ?]]]]]]]]]]]]].
     subst. eauto.
     exists (fidx func).
@@ -6786,13 +6615,13 @@ Proof.
       }
       assert (Hfds: match e with | Efun fds' _ => fds' = fds | _ => True end). {
         destruct e;auto. now inv HtopExp'. }
-      have H'' := translate_funcs_increasing_fids _ _ _ _ _ Logic.eq_refl Hfds
+      have H'' := translate_functions_increasing_fids _ _ _ _ _ Logic.eq_refl Hfds
                     Hinj Hnodup' HtransFns. clear Hfds.
       inv H.
       apply translate_fvar_fname_mapping in H1.
       destruct e; inv HtopExp'; try (now inv Hfd).
       assert (Hlen''': numOf_fundefs fds = length fns). {
-        now apply numOf_fundefs_length in HtransFns.
+        now apply translate_functions_numOf_fundefs_length in HtransFns.
       }
       rewrite Hlen''' in H1.
 
@@ -6801,7 +6630,7 @@ Proof.
 
         intros ? Hidx.
         symmetry in Hlen'''.
-        have H' := translate_funcs_idx_bounds _ _ _ _ _ _ Hlen''' HtransFns _ Hidx. apply H'.
+        have H' := translate_functions_idx_bounds _ _ _ _ _ _ Hlen''' HtransFns _ Hidx. apply H'.
         intros ? ? Hf.
         split. { now apply local_variable_mapping_gt_idx in Hf. }
         assert (HtransF: translate_var nenv
@@ -6820,7 +6649,7 @@ Proof.
       }
       assert (Hfds: match e with | Efun fds' _ => fds' = fds | _ => True end). {
         destruct e;auto. now inv HtopExp'. }
-      have H' := translate_funcs_NoDup _ _ _ _ _ Logic.eq_refl Hfds Hinj Hnodup' HtransFns.
+      have H' := translate_functions_NoDup _ _ _ _ _ Logic.eq_refl Hfds Hinj Hnodup' HtransFns.
       apply NoDup_nth_error. rewrite NoDup_nth_error in H'.
       intros. apply H'.
       - now rewrite map_length.
@@ -6873,7 +6702,7 @@ Proof.
 	replace (match e with | Efun _ exp => exp
                         | _ => e end) with e0 by now destruct e.
   reflexivity.
-  rewrite -HtransFns. destruct e; inv HtopExp'; auto.
+  rewrite -HtransFns. by destruct e; inv HtopExp'.
 Qed.
 
 Lemma repeat0_n_zeros : forall l,
@@ -6934,31 +6763,33 @@ Proof.
   assert (Hnodup: NoDup (collect_function_vars (Efun Fnil e))) by constructor.
 
   assert (Hcenv' : (forall (f : var) (t : fun_tag) (ys : seq var) (e1 : exp),
-      find_def f match
-          match e with
-          | Efun _ _ => e
-          | _ => Efun Fnil e
-          end
-        with
-        | Efun fds' _ => fds'
-        | _ => Fnil
-        end = Some (t, ys, e1) ->
+    find_def f match
+                 match e with
+                 | Efun _ _ => e
+                 | _ => Efun Fnil e
+                 end
+               with
+               | Efun fds' _ => fds'
+               | _ => Fnil
+               end = Some (t, ys, e1) ->
       correct_cenv_of_exp cenv e1)). { intros. destruct e; try discriminate. cbn in Hcenv.
       eapply Forall_constructors_subterm; try apply Hcenv. constructor. apply dsubterm_fds.
-      now eapply find_def_dsubterm_fds_e. }
+      now eapply find_def_dsubterm_fds_e.
+  }
 
   assert (Hnodup': NoDup
-       (collect_function_vars
-          (Efun match
-               match e with
-               | Efun _ _ => e
-               | _ => Efun Fnil e
-               end
-             with
-             | Efun fds' _ => fds'
-             | _ => Fnil
-             end e))). { destruct e; cbn; auto.
-                         now eapply NoDup_app_remove_l in HvarsNodup. }
+    (collect_function_vars (Efun match
+                                   match e with
+                                   | Efun _ _ => e
+                                   | _ => Efun Fnil e
+                                   end
+                                 with
+                                 | Efun fds' _ => fds'
+                                 | _ => Fnil
+                                 end e))). {
+    destruct e; cbn; auto.
+    now eapply NoDup_app_remove_l in HvarsNodup.
+  }
 
   have HI := module_instantiate_INV_and_more_hold _ _ _ _ _ _ _ _ _ _ _ Hnodup' HeRestr
                Logic.eq_refl Logic.eq_refl Hcenv' Logic.eq_refl Hmaxfuns LANF2Wasm HflocsNil Hinst.
